rr_frontend/radium/src/lib.rs
@@ -1,5 +1,6 @@
 #![feature(box_patterns)]
 #![feature(stmt_expr_attributes)]
+#![feature(iterator_try_collect)]
 
 pub mod code;
 pub mod coq;
