stdlib/iterator/src/adapters/map.rs
@@ -36,9 +36,9 @@ impl<I, F> Map<I, F>
 
 /// Spec: We have the pure parts of the inner Next and the pre- and postconditions.
 #[rr::instantiate("Next" := "(λ π s1 e s2, 
-        if_iNone e (boringly ({MI::Next} π s1.(map_it) None s2.(map_it))) ∗
+        if_iNone e ({MI::Next} π s1.(map_it) None s2.(map_it)) ∗
         if_iSome e (λ e, ∃ e_inner,
-            boringly ({MI::Next} π s1.(map_it) (Some e_inner) s2.(map_it)) ∗
+            ({MI::Next} π s1.(map_it) (Some e_inner) s2.(map_it)) ∗
             boringly ({MF::Pre} π s1.(map_clos) *[e_inner]) ∗
             boringly ({MF::PostMut} π s1.(map_clos) *[e_inner] s2.(map_clos) e)
             ))%I")]
