case_studies/refinedrust-20-paper-examples/extra_specs.v
@@ -2,16 +2,16 @@ Section extra_specs.
 Context `{RRGS : !refinedrustGS Σ}.
 
 (* Proved by manual induction: inductive property about the emitted elements *)
-Global Program Instance learn_from_hyp_list_it π T_rt s1 hist s2 :
-  LearnFromHyp (IteratorNextFusedTrans (ListIteraTasstd_iter_Iterator_spec_attrs T_rt) π s1 hist s2) :=
-  {| learn_from_hyp_Q := ⌜s1 = hist ++ s2⌝%I |}.
+Global Program Instance iterator_learn_list T_rt :
+  IteratorLearnInductive (ListIteraTasstd_iter_Iterator_spec_attrs T_rt) :=
+  {| iterator_learn_inductive_Q s1 hist s2 := s1 = hist ++ s2 |}.
 Next Obligation.
-  iIntros (???????) "Hx".
-  iModIntro.
+  iIntros (?????) "Hx".
+  iPoseProof (boringly_persistent_elim with "Hx") as "Hx".
   iInduction hist as [ | x hist] "IH" forall (s1 s2); simpl.
   { iDestruct "Hx" as "->". iPureIntro. done. } 
   iDestruct "Hx" as "(%s1' & (_ & ->) & Hx)".
-  iPoseProof ("IH" with "Hx") as "($ & ->)".
+  iPoseProof ("IH" with "Hx") as "->".
   done.
 Qed.
 
