stdlib/iterator/extra_specs.v
@@ -1,0 +1,212 @@
+Section extra.
+ Context `{RRGS : !refinedrustGS Σ}.
+
+  Lemma iterator_next_fused_trans_map_inv {MB_rt MI_rt MF_rt Item_rt}
+  (It_attrs : traits_iterator_Iterator_spec_attrs MI_rt Item_rt)
+  (FnOnce_attrs : FnOnce_spec_attrs MF_rt (tuple1_rt Item_rt) MB_rt)
+  (FnMut_attrs : FnMut_spec_attrs MF_rt (tuple1_rt Item_rt) MB_rt) π s1 hist s2 :
+    IteratorNextFusedTrans (adapters_map_MapMIMFastraits_iterator_Iterator_spec_attrs MB_rt MI_rt MF_rt Item_rt It_attrs FnOnce_attrs FnMut_attrs) π s1 hist s2 -∗
+    ∃ hist' states,
+      ⌜states !! 0%nat = Some s1.(map_clos)⌝ ∗
+      ⌜states !! (length hist) = Some s2.(map_clos)⌝ ∗
+      ⌜length states = S (length hist)⌝ ∗
+      IteratorNextFusedTrans It_attrs π s1.(map_it) hist' s2.(map_it) ∗
+      [∗ list] i ↦ a; b ∈ hist'; hist,
+        ∃ s1 s2, ⌜states !! i = Some s1⌝ ∗ ⌜states !! S i = Some s2⌝ ∗ ☒ FnOnce_attrs.(FnOnce_Pre) π s1 *[a] ∗ ☒ FnMut_attrs.(FnMut_PostMut) π s1 *[a] s2 b
+  .
+  Proof.
+    iInduction hist as [ | a hist] "IH" forall (s1 s2); simpl.
+    { iIntros "<-". iExists [], [s1.(map_clos)]. simpl. done. }
+    iIntros "(%s1' & (_ & %b & Ha & Hpre & Hpost) & Hc)".
+    iPoseProof ("IH" with "Hc") as "(%hist' & %states & % & % & %Hlen & Hit & Hclos)".
+    iExists (b :: hist'), (s1.(map_clos) :: states).
+    iR.
+    iSplitR. { iPureIntro. simpl. done. }
+    iSplitR. { iPureIntro. simpl. rewrite Hlen. done. }
+    simpl. iFrame "Hclos".
+    iFrame. done.
+  Qed.
+
+
+  (** Declared as an extern instance below, to enforce order on the argument resolution *)
+  Program Definition iterator_learn_map_stateless {MB_rt MI_rt MF_rt Item_rt}
+  (It_attrs : traits_iterator_Iterator_spec_attrs MI_rt Item_rt)
+  (FnOnce_attrs : FnOnce_spec_attrs MF_rt (tuple1_rt Item_rt) MB_rt)
+  (FnMut_attrs : FnMut_spec_attrs MF_rt (tuple1_rt Item_rt) MB_rt)
+  (It_learn : IteratorLearnInductive It_attrs)
+
+  (FnOnce_pre_learn : ∀ π self args, SimplifyBoringlyImpl (FnOnce_attrs.(FnOnce_Pre) π self args))
+  (FnMut_postmut_learn : ∀ π self args self' out, SimplifyBoringlyImpl (FnMut_attrs.(FnMut_PostMut) π self args self' out))
+  (FnMut_postmut_stateless : ∀ π args out, RelationIsIdentity (λ self self', (FnMut_postmut_learn π self args self' out).(simplify_boringly_impl_q _)))
+  :
+    IteratorLearnInductive (adapters_map_MapMIMFastraits_iterator_Iterator_spec_attrs MB_rt MI_rt MF_rt Item_rt It_attrs FnOnce_attrs FnMut_attrs) := {|
+      iterator_learn_inductive_Q s1 hist s2 :=
+        ∃ π hist',
+          It_learn.(iterator_learn_inductive_Q) s1.(map_it) hist' s2.(map_it) ∧
+          s1.(map_clos) = s2.(map_clos) ∧
+          Forall2 (λ a b, (FnOnce_pre_learn π s1.(map_clos) *[a]).(simplify_boringly_impl_q _) ∧ (FnMut_postmut_learn π s1.(map_clos) *[a] s1.(map_clos) b).(simplify_boringly_impl_q _)) hist' hist
+        ;
+    |}.
+  Next Obligation.
+    intros ???? It_attrs FnOnce_attrs FnMut_attrs It_learn FnOnce_pure FnMut_pure FnMut_stateless.
+    simpl. iIntros (? s1 hist s2) "Hnext".
+    iPoseProof (boringly_mono with "Hnext") as "Ha".
+    { iApply iterator_next_fused_trans_map_inv. }
+    repeat setoid_rewrite boringly_exists.
+    iDestruct "Ha" as "(%hist' & %states' & Ha)".
+    rewrite !boringly_sep !boringly_persistent_elim.
+    iDestruct "Ha" as "(%Hlook1 & %Hlook2 & %Hlen & Hnext & Hclos)".
+    iPoseProof (It_learn.(iterator_learn_inductive_proof) with "Hnext") as "%Hlearn".
+
+    iAssert (⌜∀ i x y, states' !! i = Some x → states' !! (S i) = Some y → x = y⌝)%I as "%Hstates".
+    { iIntros (i ? ? Hlook3 Hlook4). iClear "Hnext".
+      assert (i < length hist). { apply lookup_lt_Some in Hlook4. lia. }
+      iPoseProof (big_sepL2_length with "Hclos") as "%Hlen'".
+      odestruct (lookup_lt_is_Some_2 hist i _) as (sb & ?); first lia.
+      odestruct (lookup_lt_is_Some_2 hist' i _) as (sa & ?). { rewrite Hlen'. lia. }
+
+      iPoseProof (big_sepL2_lookup _ _ _ i sa sb with "Hclos") as "Ha"; [done.. | ].
+      iDestruct "Ha" as "(% & % & % & % & Hpre & Hpost)".
+
+      rewrite ((FnMut_pure π _ _ _ _).(simplify_boringly_impl_proof)).
+      iDestruct "Hpost" as "%Hpost".
+      apply FnMut_stateless in Hpost.
+      simplify_eq. done. }
+    (* prove that the state remains constant *)
+    assert (∀ j i s, (i < j)%nat → states' !! i = Some s → s = s1.(map_clos)) as Hstates'.
+    { clear -Hstates Hlook1.
+      induction j as [ | j IH]; simpl in *. { intros. lia. }
+      intros i s Hlt Hlook.
+      apply lookup_lt_Some in Hlook as ?.
+      destruct (decide (i = j)) as [-> | ?].
+      - destruct j as [ | j]; first by simplify_eq.
+        odestruct (lookup_lt_is_Some_2 states' j _) as (? & Hlook2); first lia.
+        ospecialize (IH j _ _ _); [lia | done | ].
+        subst. symmetry. by eapply (Hstates j).
+      - eapply IH; last done. lia. }
+
+    iExists π, hist'.
+    iSplitR; first done.
+    iSplitR. { iPureIntro. symmetry. eapply (Hstates' (S (length hist))); last done. lia. }
+    iApply big_sepL2_Forall2.
+    iApply (big_sepL2_impl with "Hclos").
+    iModIntro. iIntros (? ?? Hlook3 Hlook4) "(%sa & %sb & %Hlook5 & %Hlook6 & Hpre & Hpost)".
+    rewrite ((FnMut_pure _ _ _ _ _).(simplify_boringly_impl_proof)).
+    rewrite ((FnOnce_pure _ _ _).(simplify_boringly_impl_proof)).
+    iDestruct "Hpre" as "%".
+    iDestruct "Hpost" as "%".
+    opose proof (Hstates' (S k) k _ _ Hlook5); first lia.
+    opose proof (Hstates' (S (S k)) (S k) _ _ Hlook6); first lia.
+    subst. done.
+  Qed.
+
+  Program Definition iterator_learn_range_it
+    (Clone_attrs : Clone_spec_attrs Z)
+    (PartialEq_attrs : PartialEq_spec_attrs Z Z)
+    (PartialOrd_attrs : PartialOrd_spec_attrs Z Z PartialEq_attrs)
+    (Step_attrs : step_Step_spec_attrs Z Clone_attrs PartialEq_attrs PartialOrd_attrs)
+    :
+    (∀ a b z, Step_attrs.(step_Step_Forward) a b = Some z → z = a + b) →
+    (∀ a b, PartialOrd_attrs.(PartialOrd_POrd) a b = Some (Z.cmp a b)) →
+    IteratorLearnInductive (step_impltraits_iterator_Iteratorforstd_ops_RangeA_spec_attrs (Z)
+      Clone_attrs PartialEq_attrs PartialOrd_attrs Step_attrs) :=
+    λ _ _, {| iterator_learn_inductive_Q s1 hist s2 :=
+        s1.2 = s2.2 ∧ s1.1 ≤ s2.1 ∧ hist = seqZ s1.1 (s2.1 - s1.1) |}.
+  Next Obligation.
+    iIntros (???? Hstep Hcmp_eq ????) "Hx".
+    iPoseProof (boringly_persistent_elim with "Hx") as "Hx".
+    iInduction hist as [ | x hist] "IH" forall (s1 s2); simpl.
+    { iDestruct "Hx" as "%". subst. iPureIntro.
+      rewrite Z.sub_diag. done. }
+    iDestruct "Hx" as "(%s1' & %Ha & Hx)".
+    iPoseProof ("IH" with "Hx") as "%Hb".
+    iPureIntro.
+    destruct Ha as (? & _ & <- & Hstep_some & Hcmp). destruct Hb as (? & ? & ->).
+    destruct s1, s2, s1'; simpl in *.
+    subst.
+    symmetry in Hstep_some. apply Hstep in Hstep_some.
+    subst z.
+    rewrite Hcmp_eq in Hcmp.
+    injection Hcmp.
+    rewrite Z.cmp_less_iff. intros.
+    split_and!; try solve_goal.
+    rewrite (seqZ_cons r (r1 - r)); last lia.
+    f_equiv. f_equiv; lia.
+  Qed.
+
+
+  Program Definition iterator_learn_range_it_i8 :=
+    iterator_learn_range_it (i8asClone_spec_attrs) (i8asPartialEq_spec_attrs) (i8asPartialOrd_spec_attrs) (i8asstep_Step_spec_attrs) _ _.
+  Next Obligation. simpl; intros; case_bool_decide; simplify_eq; done. Qed.
+  Next Obligation. done. Qed.
+  Global Existing Instance iterator_learn_range_it_i8.
+
+  Program Definition iterator_learn_range_it_i16 :=
+    iterator_learn_range_it (i16asClone_spec_attrs) (i16asPartialEq_spec_attrs) (i16asPartialOrd_spec_attrs) (i16asstep_Step_spec_attrs) _ _.
+  Next Obligation. simpl; intros; case_bool_decide; simplify_eq; done. Qed.
+  Next Obligation. done. Qed.
+  Global Existing Instance iterator_learn_range_it_i16.
+
+  Program Definition iterator_learn_range_it_i32 :=
+    iterator_learn_range_it (i32asClone_spec_attrs) (i32asPartialEq_spec_attrs) (i32asPartialOrd_spec_attrs) (i32asstep_Step_spec_attrs) _ _.
+  Next Obligation. simpl; intros; case_bool_decide; simplify_eq; done. Qed.
+  Next Obligation. done. Qed.
+  Global Existing Instance iterator_learn_range_it_i32.
+
+  Program Definition iterator_learn_range_it_i64 :=
+    iterator_learn_range_it (i64asClone_spec_attrs) (i64asPartialEq_spec_attrs) (i64asPartialOrd_spec_attrs) (i64asstep_Step_spec_attrs) _ _.
+  Next Obligation. simpl; intros; case_bool_decide; simplify_eq; done. Qed.
+  Next Obligation. done. Qed.
+  Global Existing Instance iterator_learn_range_it_i64.
+
+  Program Definition iterator_learn_range_it_i128 :=
+    iterator_learn_range_it (i128asClone_spec_attrs) (i128asPartialEq_spec_attrs) (i128asPartialOrd_spec_attrs) (i128asstep_Step_spec_attrs) _ _.
+  Next Obligation. simpl; intros; case_bool_decide; simplify_eq; done. Qed.
+  Next Obligation. done. Qed.
+  Global Existing Instance iterator_learn_range_it_i128.
+
+  Program Definition iterator_learn_range_it_isize :=
+    iterator_learn_range_it (isizeasClone_spec_attrs) (isizeasPartialEq_spec_attrs) (isizeasPartialOrd_spec_attrs) (isizeasstep_Step_spec_attrs) _ _.
+  Next Obligation. simpl; intros; case_bool_decide; simplify_eq; done. Qed.
+  Next Obligation. done. Qed.
+  Global Existing Instance iterator_learn_range_it_isize.
+
+  Program Definition iterator_learn_range_it_u8 :=
+    iterator_learn_range_it (u8asClone_spec_attrs) (u8asPartialEq_spec_attrs) (u8asPartialOrd_spec_attrs) (u8asstep_Step_spec_attrs) _ _.
+  Next Obligation. simpl; intros; case_bool_decide; simplify_eq; done. Qed.
+  Next Obligation. done. Qed.
+  Global Existing Instance iterator_learn_range_it_u8.
+
+  Program Definition iterator_learn_range_it_u16 :=
+    iterator_learn_range_it (u16asClone_spec_attrs) (u16asPartialEq_spec_attrs) (u16asPartialOrd_spec_attrs) (u16asstep_Step_spec_attrs) _ _.
+  Next Obligation. simpl; intros; case_bool_decide; simplify_eq; done. Qed.
+  Next Obligation. done. Qed.
+  Global Existing Instance iterator_learn_range_it_u16.
+
+  Program Definition iterator_learn_range_it_u32 :=
+    iterator_learn_range_it (u32asClone_spec_attrs) (u32asPartialEq_spec_attrs) (u32asPartialOrd_spec_attrs) (u32asstep_Step_spec_attrs) _ _.
+  Next Obligation. simpl; intros; case_bool_decide; simplify_eq; done. Qed.
+  Next Obligation. done. Qed.
+  Global Existing Instance iterator_learn_range_it_u32.
+
+  Program Definition iterator_learn_range_it_u64 :=
+    iterator_learn_range_it (u64asClone_spec_attrs) (u64asPartialEq_spec_attrs) (u64asPartialOrd_spec_attrs) (u64asstep_Step_spec_attrs) _ _.
+  Next Obligation. simpl; intros; case_bool_decide; simplify_eq; done. Qed.
+  Next Obligation. done. Qed.
+  Global Existing Instance iterator_learn_range_it_u64.
+
+  Program Definition iterator_learn_range_it_u128 :=
+    iterator_learn_range_it (u128asClone_spec_attrs) (u128asPartialEq_spec_attrs) (u128asPartialOrd_spec_attrs) (u128asstep_Step_spec_attrs) _ _.
+  Next Obligation. simpl; intros; case_bool_decide; simplify_eq; done. Qed.
+  Next Obligation. done. Qed.
+  Global Existing Instance iterator_learn_range_it_u128.
+
+  Program Definition iterator_learn_range_it_usize :=
+    iterator_learn_range_it (usizeasClone_spec_attrs) (usizeasPartialEq_spec_attrs) (usizeasPartialOrd_spec_attrs) (usizeasstep_Step_spec_attrs) _ _.
+  Next Obligation. simpl; intros; case_bool_decide; simplify_eq; done. Qed.
+  Next Obligation. done. Qed.
+  Global Existing Instance iterator_learn_range_it_usize.
+
+End extra.
+Global Hint Extern 100 (IteratorLearnInductive (adapters_map_MapMIMFastraits_iterator_Iterator_spec_attrs _ _ _ _ _ _ _)) =>
+  unshelve notypeclasses refine (iterator_learn_map_stateless _ _ _ _ _ _ _); [tc_solve | tc_solve | tc_solve | tc_solve] : typeclass_instances.
